new_example/proof/person_proof.v
@@ -1,0 +1,136 @@
+From New.proof Require Import proof_prelude.
+From New.proof Require Import github_com.tchajed.marshal.
+From New.proof Require Import github_com.goose_lang.std.
+From New.code Require Import github_com.mjschwenne.grackle.new_example.
+From Grackle.pg Require Import github_com.mjschwenne.grackle.new_example.
+
+Module Person_Proof.
+  Section Status_Proof.
+
+    Context `{hG: heapGS Σ, !ffi_semantics _ _}.
+    Context `{!goGlobalsGS Σ}.
+
+    #[global]
+      Program Instance : IsPkgInit main :=
+      ltac2:(build_pkg_init ()).
+
+    Inductive V :=
+      | STATUS_UNSPECIFIED
+      | STATUS_STUDENT
+      | STATUS_STAFF
+      | STATUS_PROFESSOR.
+
+    Definition to_tag (status:V) : u64 :=
+      match status with
+      | STATUS_UNSPECIFIED => 0
+      | STATUS_STUDENT => 1
+      | STATUS_STAFF => 2
+      | STATUS_PROFESSOR => 3
+      end.
+
+    Definition to_v (status:V) := #(to_tag status).
+
+    Record C :=
+      mkC {
+        status' : V;
+      }.
+
+    Definition has_encoding (encoded:list u8) (args:C) : Prop :=
+      encoded = (u64_le (to_tag args.(status'))).
+      
+    Definition own (args__v:main.Person_Status.t) (args__c:C) (dq:dfrac) : iProp Σ :=
+      "%Hstatus" ∷ ⌜ args__v.(main.Person_Status.status') = (to_tag args__c.(status')) ⌝.
+
+    Lemma wp_GetStatus (args__t:main.Person_Status.t) (args__c:C) (dq:dfrac):
+      {{{
+            is_pkg_init main ∗
+            own args__t args__c dq
+      }}}
+        args__t @ main @ "Person_Status" @ "GetStatus" #()
+      {{{
+            status, RET #status;
+            ⌜ status = (to_tag args__c.(status')) ⌝ ∗
+            own args__t args__c dq
+      }}}.
+
+    Proof.
+      wp_start as "Hown". wp_auto.
+      iDestruct "Hown" as "%Hown".
+      iApply "HΦ".
+      iSplitR; first done.
+      done.
+    Qed.
+
+    Lemma wp_SetStatus (args__t:main.Person_Status.t) (args__c:C) new (dq:dfrac):
+      {{{
+            is_pkg_init main
+      }}}
+        args__t @ main @ "Person_Status" @ "SetStatus" #new
+      {{{
+            RET #();
+            ⌜ args__t.(main.Person_Status.status') = new ⌝ ∗
+            own args__t args__c dq
+      }}}.
+
+    Proof.
+      wp_start. wp_auto.
+      wp_if_destruct.
+      + wp_auto. iApply "HΦ".
+        iSplitL.
+    Admitted.
+      
+    Lemma wp_Enocde (args__t:main.Person_Status.t) (args__c:C) (pre_sl:slice.t) (prefix:list u8) (dq:dfrac):
+      {{{
+            is_pkg_init main ∗
+            own args__t args__c dq ∗
+            own_slice pre_sl (DfracOwn 1) prefix ∗
+            own_slice_cap w8 pre_sl (DfracOwn 1)
+      }}}
+        main @ "MarshalPersonStatus" #pre_sl #args__t
+      {{{
+            enc enc_sl, RET #enc_sl;
+            ⌜ has_encoding enc args__c ⌝ ∗
+            own args__t args__c dq ∗
+            own_slice enc_sl (DfracOwn 1) (prefix ++ enc) ∗
+            own_slice_cap w8 enc_sl (DfracOwn 1)
+      }}}.
+      
+    Proof.
+      wp_start as "(Hown & Hsl & Hcap)". wp_auto.
+      iDestruct "Hown" as "%Hown_status".
+
+      wp_apply (wp_WriteInt with "[$Hsl $Hcap]").
+      iIntros (?) "[Hsl Hcap]". wp_auto.
+
+      iApply "HΦ". iFrame.
+      iSplit.
+      + iPureIntro. unfold has_encoding. rewrite Hown_status. reflexivity.
+      + done.
+    Qed.
+
+    Lemma wp_Decode (enc: list u8) (enc_sl: slice.t) (args__c:C) (suffix: list u8) (dq: dfrac):
+      {{{
+            is_pkg_init main ∗
+            own_slice enc_sl dq (enc ++ suffix) ∗
+            ⌜ has_encoding enc args__c ⌝
+      }}}
+        main @ "UnmarshalPersonStatus" #enc_sl
+      {{{
+            args__t suff_sl, RET (#args__t, #suff_sl);
+            own args__t args__c (DfracOwn 1) ∗
+            own_slice suff_sl dq suffix
+      }}}.
+
+    Proof.
+      wp_start as "(Hsl & %Henc)". wp_auto.
+      unfold has_encoding in Henc.
+      rewrite Henc.
+
+      wp_apply (wp_ReadInt with "[$Hsl]").
+      iIntros (?) "Hsl". wp_auto.
+
+      wp_apply (wp_SetStatus with "[status]").
+      iIntros "[%Hstatus Hown]". wp_auto.
+    Admitted.
+  End Status_Proof.
+End Person_Proof.
